Dataflow/MemSemantics.v
@@ -99,7 +99,7 @@ Module Type MEMSEMANTICS
              clock_of xss bk ->
              find_node f G = Some (mk_node f i o v eqs) ->
              (exists H,
-                 sem_vars bk H (Nelist.nefst i) xss
+                 sem_vars bk H (Nelist.map_fst i) xss
                  /\ sem_var bk H (fst o) ys
                  /\ (forall n, absent_list xss n <-> ys n = absent)
                  /\ Forall (msem_equation G bk H M) eqs) ->
@@ -188,12 +188,12 @@ enough: it does not support the internal fixpoint introduced by
              (Hbk : clock_of xss bk)
              (Hfind : find_node f G = Some (mk_node f i o v eqs))
              (Hnode : exists H : history,
-                 sem_vars bk H (Nelist.nefst i) xss
+                 sem_vars bk H (Nelist.map_fst i) xss
                  /\ sem_var bk H (fst o) ys
                  /\ (forall n, absent_list xss n <-> ys n = absent)
                  /\ Forall (msem_equation G bk H M) eqs),
         (exists H : history,
-            sem_vars bk H (Nelist.nefst i) xss
+            sem_vars bk H (Nelist.map_fst i) xss
             /\ sem_var bk H (fst o) ys
             /\ (forall n, absent_list xss n <-> ys n = absent)
             /\ Forall (fun eq=>exists Hsem, P (bk := bk) (eq := eq)(M := M)(H := H) Hsem) eqs)
