DataflowToClight.v
@@ -3,14 +3,14 @@ Require Import Rustre.Dataflow.
 Require Import Rustre.Dataflow.IsFree.Decide.
 Require Import Rustre.Dataflow.WellFormed.Decide.
 Require Import Rustre.Interface.
-Require Import Rustre.DF2MP.Translation.
-Require Import Rustre.MP2CL.Translation.
+Require Import Rustre.DataflowToMinimp.Translation.
+Require Import Rustre.MinimpToClight.Translation.
 Require Import Rustre.Minimp.FuseIfte.
 
 Require Import common.Errors.
 
 Module Import SynDF := Dataflow.Syntax.SyntaxFun Op.
-Module Import SynMP := MP2CL.Translation.Syn.
+Module Import SynMP := MinimpToClight.Translation.Syn.
 Module Import DF2MPTrans := TranslationFun Op SynDF SynMP.
 
 Module Import IsF := IsFreeFun Op SynDF.
@@ -25,7 +25,7 @@ Module Import WefD := Dataflow.WellFormed.Decide.DecideFun Op SynDF IsF IsFDec O
 
 Module Import SemMP := Rustre.Minimp.Semantics.SemanticsFun Op SynMP.
 Module Import Equ := Rustre.Minimp.Equiv.EquivFun Op SynMP SemMP.
-Module Import FuseIFTE := FuseIfteFun Op SynDF MP2CL.Translation.Syn SemMP Equ.
+Module Import FuseIFTE := FuseIfteFun Op SynDF MinimpToClight.Translation.Syn SemMP Equ.
 
 Require Import String.
 
@@ -35,7 +35,7 @@ Definition is_well_sch (res: Errors.res unit) (n: node) :=
   match res with
   | OK _ =>
     let eqs := n.(n_eqs) in
-    let ni := Nelist.nefst n.(n_input) in
+    let ni := Nelist.map_fst n.(n_input) in
     if well_sch (memories eqs) ni eqs then OK tt
     else Error (Errors.msg ("node " ++ pos_to_str n.(n_name) ++ " is not well scheduled."))
   | _ => res
@@ -49,4 +49,4 @@ Definition fuse (c: class): class :=
 
 Definition compile (g: global) (main_node: ident) :=
   do _ <- (List.fold_left is_well_sch g (OK tt));
-  MP2CL.Translation.translate (List.map fuse (DF2MPTrans.translate g)) main_node.
+  MinimpToClight.Translation.translate (List.map fuse (DF2MPTrans.translate g)) main_node.
