MinimpToClight/Correctness.v
@@ -1,0 +1,174 @@
+Set Automatic Coercions Import.
+
+Require Import Rustre.Common.
+Require Import Rustre.MP2CL.Translation.
+Require Import Rustre.Minimp.Semantics.
+Require Import Rustre.Interface.
+
+Module Import Sem := SemanticsFun Op Syn.
+
+Require Import common.Events.
+Require Import common.Globalenvs.
+Require Import common.Memory.
+Require Import lib.Integers.
+Require Import common.Smallstep.
+Require Import common.Errors.
+Require Import lib.Coqlib.
+Require common.AST.
+Require cfrontend.Clight.
+
+Require Import Arith.Wf_nat.
+
+Open Scope list_scope.
+Import List.ListNotations.
+
+Record fundef := Fundef {name: ident; body: stmt}.
+Definition vardef := cl_ident.
+
+Definition genv := Genv.t fundef vardef.
+Inductive state := State (H: heap) (S: stack) (s: stmt).
+
+Definition make_gvar (init volatile: bool) (name: cl_ident) :=
+  (name,
+   @AST.Gvar fundef _ (AST.mkglobvar name (if init then [AST.Init_space Z0] else []) false volatile)).
+
+Definition make_gfun (name: cl_ident) (body: stmt) :=
+  (name,
+   @AST.Gfun _ vardef (Fundef name body)).
+
+Definition convert_class (defs: list (cl_ident * AST.globdef fundef vardef)) (c: class)
+  : list (cl_ident * AST.globdef fundef vardef) :=
+  match c with
+    mk_class c_name c_input c_output c_mems c_objs c_step c_reset =>
+    let name := translate_ident c_name in
+    let cls := make_gvar false false name in
+    let step := make_gfun (step_id name) c_step in
+    let reset := make_gfun (reset_id name) c_reset in
+    cls :: step :: reset :: defs
+  end.
+
+Definition convert_prog (p: program): AST.program fundef vardef :=
+  let defs := List.fold_left convert_class p nil in
+  AST.mkprogram defs [] main_id.
+  
+Inductive step: genv -> state -> trace -> state -> Prop :=
+  DoStep: forall prog ge H S s H' S' t,
+    stmt_eval prog H S s (H', S') ->
+    step ge (State H S s) t (State H' S' Skip).
+
+Definition globalenv (p: program) :=
+  Genv.globalenv (convert_prog p).
+
+Parameter convert_mem: mem -> heap * stack.
+Inductive initial_state (p: program): state -> Prop :=
+  IniState: forall b f m0 H0 S0,
+    let ge := globalenv p in
+    let p' := convert_prog p in
+    Genv.init_mem p' = Some m0 ->
+    Genv.find_symbol ge p'.(AST.prog_main) = Some b ->
+    Genv.find_funct_ptr ge b = Some f ->
+    convert_mem m0 = (H0, S0) ->
+    initial_state p (State H0 S0 f.(body)).
+
+Inductive final_state (s: state) (n: int): Prop := False.
+
+Definition semantics (p: program) :=
+  let ge := globalenv p in
+  Semantics_gen step (initial_state p) final_state ge ge.
+
+Section SPEC.
+
+  Inductive tr_function: fundef -> Clight.function -> Prop :=
+    tr_function_intro: forall f tf,
+      (* tr_stmt f.(Csyntax.fn_body) tf.(fn_body) -> *)
+      (* fn_return tf = Csyntax.fn_return f -> *)
+      (* fn_callconv tf = Csyntax.fn_callconv f -> *)
+      (* fn_params tf = Csyntax.fn_params f -> *)
+      (* fn_vars tf = Csyntax.fn_vars f -> *)
+      (* tr_function f tf *) tr_function f tf.
+
+  Inductive tr_fundef: fundef -> Clight.fundef -> Prop :=
+    tr_fundef_intro: forall f tf,
+      tr_function f tf -> tr_fundef f (Clight.Internal tf).
+
+  Inductive tr_vardef: vardef -> Ctypes.type -> Prop :=
+    tr_vardef_intro: forall x t,
+      tr_vardef x t.
+
+  Theorem transl_program_spec:
+    forall main_node p tp,
+      translate p main_node = OK tp ->
+      AST.match_program tr_fundef tr_vardef nil main_id (convert_prog p) tp.
+  Admitted.
+
+End SPEC.
+Section PRESERVATION.
+ 
+  Variable main_node : ident.
+
+  Variable prog: program.
+  Variable tprog: Clight.program.
+  Hypothesis TRANSL: translate prog main_node = OK tprog.
+  
+  Let ge := globalenv prog.
+  Let tge := Clight.globalenv tprog.
+
+  Definition measure (st: state) : nat := 0%nat.
+  
+  Inductive match_states: state -> Clight.state -> Prop :=
+    match_intro: forall S S', match_states S S'.
+
+  Lemma public_preserved:
+    forall (s: ident), Genv.public_symbol tge s = Genv.public_symbol ge s.
+  Proof.
+    intros. eapply Genv.public_symbol_match. eapply transl_program_spec; eauto.
+    simpl. tauto.
+  Qed.
+
+  (* 
+    S1 <------->    S1'
+    |t           |t or |t 
+    v            v+    v* |S2| < |S1|
+    S2 <------->    S2'
+ *)
+  Theorem simulation:
+    forall S1 t S2,
+      step ge S1 t S2 ->
+      forall S1' (MS: match_states S1 S1'),
+      exists S2',
+        (plus Clight.step1 tge S1' t S2' \/
+         (star Clight.step1 tge S1' t S2' /\ measure S2 < measure S1)%nat)
+        /\ match_states S2 S2'.
+  Proof.
+    intros S1 t S2 STEP. destruct STEP. destruct H0; admit.
+  Qed.
+  
+  Lemma transl_initial_states:
+    forall S,
+      initial_state prog S ->
+      exists S', Clight.initial_state tprog S' /\ match_states S S'.
+  Proof.
+    intros S IS. inv IS.
+    admit.
+  Qed.
+
+  Lemma transl_final_states:
+    forall S S' r,
+      match_states S S' -> final_state S r -> Clight.final_state S' r.
+  Proof.
+    intros S S' r H FS.
+    admit.
+  Qed.
+
+  Theorem transl_program_correct:
+    forward_simulation (semantics prog) (Clight.semantics1 tprog).
+  Proof.
+    eapply forward_simulation_star_wf with (order := ltof _ measure).
+    eexact public_preserved.
+    eexact transl_initial_states.
+    eexact transl_final_states.
+    apply well_founded_ltof.
+    exact simulation.
+  Qed.
+
+End PRESERVATION.
